pulse/lib/pulse/core/PulseCore.Atomic.fsti
@@ -1,9 +1,26 @@
+(*
+   Copyright 2024 Microsoft Research
+
+   Licensed under the Apache License, Version 2.0 (the "License");
+   you may not use this file except in compliance with the License.
+   You may obtain a copy of the License at
+
+       http://www.apache.org/licenses/LICENSE-2.0
+
+   Unless required by applicable law or agreed to in writing, software
+   distributed under the License is distributed on an "AS IS" BASIS,
+   WITHOUT WARRANTIES OR CONDITIONS OF ANY KIND, either express or implied.
+   See the License for the specific language governing permissions and
+   limitations under the License.
+*)
+
 module PulseCore.Atomic
+
+open FStar.Ghost
+
 open PulseCore.InstantiatedSemantics
 open PulseCore.Action
 open PulseCore.Observability
-open FStar.Ghost
-
 
 (* stt_unobservable a opens pre post: The type of a pulse computation
    that when run in a state satisfying `pre`
@@ -18,7 +35,7 @@ val stt_atomic
     (opens:inames)
     (pre:slprop)
     (post:a -> slprop)
-: Type u#(max 3 a)
+: Type u#(max 4 a)
 
 val return_atomic
     (#a:Type u#a)
@@ -123,95 +140,103 @@ val sub_invs_stt_atomic
 [@@ erasable]
 val stt_ghost
     (a:Type u#a)
+    (opens:inames)
     (pre:slprop)
     (post:a -> slprop)
-: Type u#(max 3 a)
+: Type u#(max 4 a)
 
 val return_ghost
     (#a:Type u#a)
     (x:a)
     (p:a -> slprop)
-: stt_ghost a (p x) (fun r -> p r ** pure (r == x))
+: stt_ghost a emp_inames (p x) (fun r -> p r ** pure (r == x))
 
 val return_ghost_noeq
     (#a:Type u#a)
     (x:a)
     (p:a -> slprop)
-: stt_ghost a (p x) p
+: stt_ghost a emp_inames (p x) p
 
 val bind_ghost
     (#a:Type u#a)
     (#b:Type u#b)
+    (#opens:inames)
     (#pre1:slprop)
     (#post1:a -> slprop)
     (#post2:b -> slprop)
-    (e1:stt_ghost a pre1 post1)
-    (e2:(x:a -> stt_ghost b (post1 x) post2))
-: stt_ghost b pre1 post2
+    (e1:stt_ghost a opens pre1 post1)
+    (e2:(x:a -> stt_ghost b opens (post1 x) post2))
+: stt_ghost b opens pre1 post2
 
 type non_informative_witness (a:Type u#a) =
   x:Ghost.erased a -> y:a{y == Ghost.reveal x}
 
 val lift_ghost_neutral
     (#a:Type u#a)
+    (#opens:inames)
     (#pre:slprop)
     (#post:a -> slprop)
-    (e:stt_ghost a pre post)
+    (e:stt_ghost a opens pre post)
     (reveal_a:non_informative_witness a)
-: stt_atomic a #Neutral emp_inames pre post
+: stt_atomic a #Neutral opens pre post
 
 val lift_neutral_ghost
     (#a:Type u#a)
+    (#opens:inames)
     (#pre:slprop)
     (#post:a -> slprop)
-    (e:stt_atomic a #Neutral emp_inames pre post)
-: stt_ghost a pre post
+    (e:stt_atomic a #Neutral opens pre post)
+: stt_ghost a opens pre post
 
 val frame_ghost
     (#a:Type u#a)
+    (#opens:inames)
     (#pre:slprop)
     (#post:a -> slprop)
     (frame:slprop)
-    (e:stt_ghost a pre post)
-: stt_ghost a (pre ** frame) (fun x -> post x ** frame)
+    (e:stt_ghost a opens pre post)
+: stt_ghost a opens (pre ** frame) (fun x -> post x ** frame)
 
 val sub_ghost
     (#a:Type u#a)
+    (#opens:inames)
     (#pre1:slprop)
     (pre2:slprop)
     (#post1:a -> slprop)
     (post2:a -> slprop)
     (pf1 : slprop_equiv pre1 pre2)
     (pf2 : slprop_post_equiv post1 post2)
-    (e:stt_ghost a pre1 post1)
-: stt_ghost a pre2 post2
+    (e:stt_ghost a opens pre1 post1)
+: stt_ghost a opens pre2 post2
 
 val noop (p:slprop)
-: stt_ghost unit p (fun _ -> p)
+: stt_ghost unit emp_inames p (fun _ -> p)
 
 val intro_pure (p:prop) (pf:squash p)
-: stt_ghost unit emp (fun _ -> pure p)
+: stt_ghost unit emp_inames emp (fun _ -> pure p)
 
 val elim_pure (p:prop)
-: stt_ghost (squash p) (pure p) (fun _ -> emp)
+: stt_ghost (squash p) emp_inames (pure p) (fun _ -> emp)
 
 val intro_exists (#a:Type u#a) (p:a -> slprop) (x:erased a)
-: stt_ghost unit (p x) (fun _ -> exists* x. p x)
+: stt_ghost unit emp_inames (p x) (fun _ -> exists* x. p x)
 
 val elim_exists (#a:Type u#a) (p:a -> slprop)
-: stt_ghost (erased a) (exists* x. p x) (fun x -> p x)
+: stt_ghost (erased a) emp_inames (exists* x. p x) (fun x -> p x)
 
 val ghost_reveal (a:Type) (x:erased a)
-  : stt_ghost a emp (fun y -> pure (reveal x == y))
+  : stt_ghost a emp_inames emp (fun y -> pure (reveal x == y))
 
 //////////////////////////////////////////////////////////////////
 
-val new_invariant
-    (p:slprop)
-: stt_atomic (inv p) #Unobservable emp_inames p (fun _ -> emp)
+val new_invariant (p:big_vprop)
+  : stt_ghost iname_ref emp_inames p (fun i -> i -~- p)
 
-val fresh_invariant (ctx:list allocated_name) (p:slprop)
-: stt_atomic (i:inv p { name_of_inv i `fresh_wrt` ctx }) #Unobservable emp_inames p (fun _ -> emp)
+val fresh_invariant (ctx:list iname_ref) (p:big_vprop)
+: stt_ghost (i:iname_ref { i `fresh_wrt` ctx })
+            emp_inames
+            p
+            (fun i -> i -~- p)
 
 val with_invariant
     (#a:Type)
@@ -219,34 +244,45 @@ val with_invariant
     (#fp:slprop)
     (#fp':a -> slprop)
     (#f_opens:inames)
-    (#p:slprop)
-    (i:inv p{not (mem_inv f_opens i)})
+    (#p:big_vprop)
+    (i:iname_ref { not (mem_inv f_opens i) })
     ($f:unit -> stt_atomic a #obs f_opens
+                             (p ** fp)
+                             (fun x -> p ** fp' x))
+: stt_atomic a #obs (add_inv f_opens i) ((i -~- p) ** fp) (fun x -> (i -~- p) ** fp' x)
+
+val with_invariant_g
+    (#a:Type)
+    (#fp:slprop)
+    (#fp':a -> slprop)
+    (#f_opens:inames)
+    (#p:big_vprop)
+    (i:iname_ref { not (mem_inv f_opens i) })
+    ($f:unit -> stt_ghost a f_opens
                             (p ** fp)
                             (fun x -> p ** fp' x))
-: stt_atomic a #(join_obs obs Unobservable) (add_inv f_opens i) fp fp'
+: stt_ghost a (add_inv f_opens i) ((i -~- p) ** fp) (fun x -> (i -~- p) ** fp' x)
 
 val distinct_invariants_have_distinct_names
     (#p:slprop)
     (#q:slprop)
-    (i:inv p)
-    (j:inv q)
+    (i j:iname_ref)
     (_:squash (p =!= q))
-: stt_atomic (squash (name_of_inv i =!= name_of_inv j))
-    #Unobservable
-    emp_inames 
-    emp
-    (fun _ -> emp)
+: stt_ghost
+    (squash (name_of_inv i =!= name_of_inv j))
+    emp_inames
+    ((i -~- p) ** (j -~- q))
+    (fun _ -> (i -~- p) ** (j -~- q))
 
 val invariant_name_identifies_invariant
       (p q:slprop)
-      (i:inv p)
-      (j:inv q { name_of_inv i == name_of_inv j } )
-: stt_atomic (squash (p == q /\ i == j))
-    #Unobservable
+      (i:iname_ref)
+      (j:iname_ref { name_of_inv i == name_of_inv j })
+: stt_ghost
+    (squash (p == q /\ i == j))
     emp_inames
-    emp
-    (fun _ -> emp)
+    ((i -~- p) ** (j -~- q))
+    (fun _ -> (i -~- p) ** (j -~- q))
 
 ////////////////////////////////////////////////////////////////////////
 // References
@@ -260,6 +296,7 @@ val pts_to_not_null
     (r:ref a p)
     (v:a)
 : stt_ghost (squash (not (is_ref_null r)))
+    emp_inames
     (pts_to r v)
     (fun _ -> pts_to r v)
 
@@ -306,6 +343,7 @@ val share
     (v0:FStar.Ghost.erased a)
     (v1:FStar.Ghost.erased a{composable pcm v0 v1})
 : stt_ghost unit
+    emp_inames
     (pts_to r (v0 `op pcm` v1))
     (fun _ -> pts_to r v0 ** pts_to r v1)
 
@@ -316,6 +354,7 @@ val gather
     (v0:FStar.Ghost.erased a)
     (v1:FStar.Ghost.erased a)
 : stt_ghost (squash (composable pcm v0 v1))
+    emp_inames
     (pts_to r v0 ** pts_to r v1)
     (fun _ -> pts_to r (op pcm v0 v1))
 
@@ -327,6 +366,7 @@ val ghost_alloc
     (#pcm:pcm a)
     (x:erased a{pcm.refine x})
 : stt_ghost (ghost_ref pcm)
+    emp_inames
     emp
     (fun r -> ghost_pts_to r x)
 
@@ -339,6 +379,7 @@ val ghost_read
         -> GTot (y:a{compatible p y v /\
                      FStar.PCM.frame_compatible p x v y})))
 : stt_ghost (erased (v:a{compatible p x v /\ p.refine v}))
+    emp_inames
     (ghost_pts_to r x)
     (fun v -> ghost_pts_to r (f v))
 
@@ -349,6 +390,7 @@ val ghost_write
     (x y:Ghost.erased a)
     (f:FStar.PCM.frame_preserving_upd p x y)
 : stt_ghost unit
+    emp_inames
     (ghost_pts_to r x)
     (fun _ -> ghost_pts_to r y)
 
@@ -359,6 +401,7 @@ val ghost_share
     (v0:FStar.Ghost.erased a)
     (v1:FStar.Ghost.erased a{composable pcm v0 v1})
 : stt_ghost unit
+    emp_inames
     (ghost_pts_to r (v0 `op pcm` v1))
     (fun _ -> ghost_pts_to r v0 ** ghost_pts_to r v1)
 
@@ -369,6 +412,7 @@ val ghost_gather
     (v0:FStar.Ghost.erased a)
     (v1:FStar.Ghost.erased a)
 : stt_ghost (squash (composable pcm v0 v1))
+    emp_inames
     (ghost_pts_to r v0 ** ghost_pts_to r v1)
     (fun _ -> ghost_pts_to r (op pcm v0 v1))
 
@@ -382,6 +426,7 @@ val big_pts_to_not_null
     (r:ref a p)
     (v:a)
 : stt_ghost (squash (not (is_ref_null r)))
+    emp_inames
     (big_pts_to r v)
     (fun _ -> big_pts_to r v)
 
@@ -428,6 +473,7 @@ val big_share
     (v0:FStar.Ghost.erased a)
     (v1:FStar.Ghost.erased a{composable pcm v0 v1})
 : stt_ghost unit
+    emp_inames
     (big_pts_to r (v0 `op pcm` v1))
     (fun _ -> big_pts_to r v0 ** big_pts_to r v1)
 
@@ -438,6 +484,7 @@ val big_gather
     (v0:FStar.Ghost.erased a)
     (v1:FStar.Ghost.erased a)
 : stt_ghost (squash (composable pcm v0 v1))
+    emp_inames
     (big_pts_to r v0 ** big_pts_to r v1)
     (fun _ -> big_pts_to r (op pcm v0 v1))
 
@@ -446,6 +493,7 @@ val big_ghost_alloc
     (#pcm:pcm a)
     (x:erased a{pcm.refine x})
 : stt_ghost (ghost_ref pcm)
+    emp_inames
     emp
     (fun r -> big_ghost_pts_to r x)
 
@@ -458,6 +506,7 @@ val big_ghost_read
         -> GTot (y:a{compatible p y v /\
                      FStar.PCM.frame_compatible p x v y})))
 : stt_ghost (erased (v:a{compatible p x v /\ p.refine v}))
+    emp_inames
     (big_ghost_pts_to r x)
     (fun v -> big_ghost_pts_to r (f v))
 
@@ -468,6 +517,7 @@ val big_ghost_write
     (x y:Ghost.erased a)
     (f:FStar.PCM.frame_preserving_upd p x y)
 : stt_ghost unit
+    emp_inames
     (big_ghost_pts_to r x)
     (fun _ -> big_ghost_pts_to r y)
 
@@ -478,6 +528,7 @@ val big_ghost_share
     (v0:FStar.Ghost.erased a)
     (v1:FStar.Ghost.erased a{composable pcm v0 v1})
 : stt_ghost unit
+    emp_inames
     (big_ghost_pts_to r (v0 `op pcm` v1))
     (fun _ -> big_ghost_pts_to r v0 ** big_ghost_pts_to r v1)
 
@@ -488,8 +539,9 @@ val big_ghost_gather
     (v0:FStar.Ghost.erased a)
     (v1:FStar.Ghost.erased a)
 : stt_ghost (squash (composable pcm v0 v1))
+    emp_inames
     (big_ghost_pts_to r v0 ** big_ghost_pts_to r v1)
     (fun _ -> big_ghost_pts_to r (op pcm v0 v1))
 
 val drop (p:slprop)
-: stt_ghost unit p (fun _ -> emp)
+: stt_ghost unit emp_inames p (fun _ -> emp)
