pulse/lib/pulse/core/PulseCore.NondeterministicPreorderStateMonad.fst
@@ -1,0 +1,55 @@
+(*
+   Copyright 2024 Microsoft Research
+
+   Licensed under the Apache License, Version 2.0 (the "License");
+   you may not use this file except in compliance with the License.
+   You may obtain a copy of the License at
+
+       http://www.apache.org/licenses/LICENSE-2.0
+
+   Unless required by applicable law or agreed to in writing, software
+   distributed under the License is distributed on an "AS IS" BASIS,
+   WITHOUT WARRANTIES OR CONDITIONS OF ANY KIND, either express or implied.
+   See the License for the specific language governing permissions and
+   limitations under the License.
+*)
+
+module PulseCore.NondeterministicPreorderStateMonad
+
+open FStar.Preorder
+friend PulseCore.PreorderStateMonad
+
+type tape = nat -> bool
+type ctr = nat
+
+type npst' (#s:Type u#s)
+           (a:Type u#a)
+           (rel:preorder s)
+           (pre:req_t s)
+           (post:ens_t s a) =
+  s0:s { pre s0 } ->
+  tape ->
+  ctr ->
+  Dv (res:(a & s & ctr) {
+    post s0 res._1 res._2 /\
+    rel s0 res._2
+  })
+
+let npst #s a rel pre post =
+  unit -> Dv (npst' #s a rel pre post)
+
+let lift #s #a #rel #pre #post f =
+  fun () s0 t c -> let x, s1 = f s0 in x, s1, c
+
+let return #s #rel #a x =
+  fun () s0 t c -> x, s0, c
+
+let bind #s #a #b #rel #req_f #ens_f #req_g #ens_g f g =
+  fun () s0 t c ->
+  let x, s1, c = f () s0 t c in
+  g x () s1 t c
+
+let weaken #s #rel #a #req_f #ens_f #req_g #ens_g f =
+  fun () s0 t c -> f () s0 t c
+
+let flip () = fun () s0 t c -> t c, s0, c+1
