pulse/lib/pulse/core/PulseCore.Observability.fst
@@ -1,3 +1,19 @@
+(*
+   Copyright 2024 Microsoft Research
+
+   Licensed under the Apache License, Version 2.0 (the "License");
+   you may not use this file except in compliance with the License.
+   You may obtain a copy of the License at
+
+       http://www.apache.org/licenses/LICENSE-2.0
+
+   Unless required by applicable law or agreed to in writing, software
+   distributed under the License is distributed on an "AS IS" BASIS,
+   WITHOUT WARRANTIES OR CONDITIONS OF ANY KIND, either express or implied.
+   See the License for the specific language governing permissions and
+   limitations under the License.
+*)
+
 module PulseCore.Observability
 (*
 obs > unobs >----.
@@ -15,7 +31,7 @@ neutral _, ghost a |> ghost a
 type observability =
   | Neutral
   | Observable
-  | Unobservable
+  // | Unobservable
 
 let at_most_one_observable o1 o2 =
   match o1, o2 with
@@ -24,8 +40,11 @@ let at_most_one_observable o1 o2 =
 
 let join_obs o1 o2 =
   match o1, o2 with
-  | Observable, _
-  | _, Observable -> Observable
-  | Neutral, n
-  | n, Neutral -> n
-  | _ -> Unobservable
+  | Neutral, Neutral -> Neutral
+  | _ -> Observable
+  // | Observable, _
+  // | _, Observable -> Observable
+  // | _, _
+  // | Neutral, n
+  // | n, Neutral -> n
+  // | _ -> Unobservable
